steel/Zeta.Steel.EpochMap.fsti
@@ -71,7 +71,7 @@ val create (#v:Type)
 
 (* Call the finalizer on the array only.
    Freeing every element of the array is up to the client *)
-val free (#v:Type)
+val finalize (#v:Type)
          (#c:Type)
          (#vp:M.epoch_id -> v -> c -> vprop)
          (#init:G.erased c)
